src/program_proof/simplepb/pb_roapplybackup_proof.v
@@ -1,0 +1,134 @@
+From Perennial.program_proof Require Import grove_prelude.
+From Goose.github_com.mit_pdos.gokv.simplepb Require Export pb.
+From Perennial.program_proof.simplepb Require Import pb_ghost.
+From Perennial.goose_lang.lib Require Import waitgroup.
+From iris.base_logic Require Export lib.ghost_var mono_nat.
+From iris.algebra Require Import dfrac_agree mono_list.
+From Perennial.program_proof.simplepb Require Import pb_definitions pb_marshal_proof.
+From Perennial.program_proof Require Import marshal_stateless_proof.
+From Perennial.program_proof.reconnectclient Require Import proof.
+
+Section pb_roapplybackup_proof.
+
+Context `{!heapGS Σ}.
+Context {pb_record:PBRecord}.
+
+Notation OpType := (pb_OpType pb_record).
+Notation has_op_encoding := (pb_has_op_encoding pb_record).
+Notation compute_reply := (pb_compute_reply pb_record).
+Notation pbG := (pbG (pb_record:=pb_record)).
+Notation get_rwops := (get_rwops (pb_record:=pb_record)).
+
+Context `{!waitgroupG Σ}.
+Context `{!pbG Σ}.
+
+(* Clerk specs *)
+Lemma wp_Clerk__ApplyAsBackup γ γsrv ck args_ptr (epoch nextIndex:u64) opsfull :
+  {{{
+        "#Hck" ∷ is_Clerk ck γ γsrv ∗
+        "#HepochLb" ∷ is_epoch_lb γsrv epoch ∗
+        "#Hprop_lb" ∷ is_proposal_lb γ epoch opsfull ∗
+        "#Hprop_facts" ∷ is_proposal_facts γ epoch opsfull ∗
+        "%HnextIndex" ∷ ⌜length (get_rwops opsfull) = int.nat nextIndex⌝ ∗
+
+        "#HargEpoch" ∷ readonly (args_ptr ↦[pb.RoApplyAsBackupArgs :: "epoch"] #epoch) ∗
+        "#HargIndex" ∷ readonly (args_ptr ↦[pb.RoApplyAsBackupArgs :: "nextIndex"] #nextIndex)
+  }}}
+    Clerk__RoApplyAsBackup #ck #args_ptr
+  {{{
+        (err:u64), RET #err; □ if (decide (err = 0)) then
+                               is_accepted_lb γsrv epoch opsfull
+                             else True
+  }}}.
+Proof.
+  iIntros (Φ) "Hpre HΦ".
+  iNamed "Hpre".
+  wp_call.
+  wp_apply (wp_ref_of_zero).
+  { done. }
+  iIntros (rep) "Hrep".
+  wp_pures.
+  iNamed "Hck".
+  wp_apply (RoApplyAsBackupArgs.wp_Encode with "[]").
+  {
+    instantiate (1:=(RoApplyAsBackupArgs.mkC _ _)).
+    iFrame "#".
+  }
+  iIntros (enc_args enc_args_sl) "(%Henc_args & Henc_args_sl)".
+  wp_loadField.
+  iDestruct (is_slice_to_small with "Henc_args_sl") as "Henc_args_sl".
+  wp_apply (wp_frame_wand with "HΦ").
+  rewrite is_pb_host_unfold.
+  iNamed "Hsrv".
+  wp_apply (wp_ReconnectingClient__Call2 with "Hcl_rpc [] Henc_args_sl Hrep").
+  {
+    iDestruct "Hsrv" as "(_ & _ & _ & _ & _ & $ & _)".
+  }
+  { (* Successful RPC *)
+    iModIntro.
+    iNext.
+    unfold RoApplyAsBackup_spec.
+    iExists _, _.
+    iSplitR; first done.
+    iFrame "#%".
+    iSplit.
+    { (* No error from RPC, Apply was accepted *)
+      iIntros "#Hacc_lb".
+      iIntros (?) "%Henc_rep Hargs_sl".
+      iIntros (?) "Hrep Hrep_sl".
+      wp_pures.
+      wp_load.
+
+      (* FIXME: separate lemma *)
+      wp_call.
+      rewrite Henc_rep.
+      wp_apply (wp_ReadInt with "Hrep_sl").
+      iIntros (?) "_".
+      wp_pures.
+      iModIntro.
+      iIntros "HΦ".
+      iApply "HΦ".
+      iModIntro.
+      iFrame "#".
+    }
+    { (* Apply was rejected by the server (e.g. stale epoch number) *)
+      iIntros (err) "%Herr_nz".
+      iIntros.
+      wp_pures.
+      wp_load.
+      wp_call.
+      rewrite H.
+      wp_apply (wp_ReadInt with "[$]").
+      iIntros.
+      wp_pures.
+      iModIntro.
+      iIntros "HΦ".
+      iApply "HΦ".
+      iFrame.
+      iModIntro.
+      destruct (decide _).
+      {
+        exfalso. done.
+      }
+      {
+        done.
+      }
+    }
+  }
+  { (* RPC error *)
+    iIntros.
+    wp_pures.
+    wp_if_destruct.
+    {
+      iModIntro.
+      iIntros "HΦ".
+      iApply "HΦ".
+      destruct (decide (_)).
+      { exfalso. done. }
+      { done. }
+    }
+    { exfalso. done. }
+  }
+Qed.
+
+End pb_roapplybackup_proof.
